thys/Substitution/Expression_Like.thy
@@ -2,9 +2,70 @@ theory Expression_Like
   imports "Binders.MRBNF_Recursor"
 begin
 
+(**************************)
+(* 1. Preliminaries *)
+
 declare supp_id_bound[simp] supp_inv_bound[simp] infinite_UNIV[simp]
 
 definition "IImsupp' Inj Vr \<rho> = SSupp Inj \<rho> \<union> IImsupp Inj Vr \<rho>"
+
+term curry
+definition "uncurry f \<equiv> \<lambda>(a,b). f a b" 
+lemma uncorry_apply[simp]: "uncurry f (a,b) = f a b"
+  unfolding uncurry_def by auto
+
+lemma fst_comp_id[simp]: "fst \<circ> (\<lambda>e. (e, p)) = id" by auto
+
+lemma tri_Un1: "A \<subseteq> B \<union> C \<Longrightarrow> A \<union> B \<subseteq> B \<union> C" by auto
+lemma tri_Un3: "A \<union> A' \<union> A'' \<subseteq> B \<union> C \<Longrightarrow> B \<union> A \<union> A' \<union> A'' \<subseteq> B \<union> C" by auto
+
+lemma A_Int_Un_emp: "A \<inter> (B \<union> C) = {} \<longleftrightarrow> A \<inter> B = {} \<and> A \<inter> C = {}" by auto
+
+lemma bij_inv_Un_triv: "bij \<sigma> \<Longrightarrow> \<sigma> ` A \<inter> B = {} \<longleftrightarrow> A \<inter> inv \<sigma> ` B = {}"
+  by (metis bij_def empty_is_image image_Int image_inv_f_f surj_imp_inj_inv)
+
+lemma bij_in_inv_Un_triv: "bij \<sigma> \<Longrightarrow> inv \<sigma> a \<in> B \<longleftrightarrow> a \<in> \<sigma> ` B"
+  by (metis bij_inv_eq_iff imageE image_eqI)
+
+lemma incl_Un_triv3: "A1 \<union> A2 \<union> A3 \<subseteq> A \<Longrightarrow> A1 \<subseteq> A \<and> A2 \<subseteq> A \<and> A3 \<subseteq> A" by auto
+
+lemma incl_Un3_triv3: "A1 \<subseteq> B1 \<Longrightarrow> A2 \<subseteq> B2 \<union> P \<Longrightarrow> A3 \<subseteq> B3 \<union> P \<Longrightarrow> A1 \<union> A2 \<union> A3 \<subseteq> B1 \<union> B2 \<union> B3 \<union> P" 
+by auto
+
+lemma triv_Un4_remove: "A1 \<union> A2 \<union> A3 \<subseteq> B1 \<union> B2 \<union> B3 \<union> P \<Longrightarrow> A1 \<union> A2 \<union> A3 \<union> P \<subseteq> B1 \<union> B2 \<union> B3 \<union> P"
+by auto
+
+definition small :: "('a::var \<Rightarrow> 'a) \<Rightarrow> bool" where 
+"small \<sigma> \<equiv> countable (supp \<sigma>)" 
+
+declare supp_id[simp,intro] (*: "supp id = {}" unfolding supp_def by auto *)
+lemma small_id[simp,intro]: "small id" unfolding small_def by auto
+lemma supp_id'[simp,intro]: "supp (\<lambda>a. a) = {}" unfolding supp_def by auto
+lemma small_id'[simp,intro]: "small (\<lambda>a. a)" unfolding small_def by auto
+
+thm supp_o
+(* lemma supp_o: "supp (\<sigma> o \<tau>) \<subseteq> supp \<sigma> \<union> supp \<tau>" unfolding supp_def by auto *)
+lemma small_o[simp]: "small \<sigma> \<Longrightarrow> small \<tau> \<Longrightarrow> small (\<sigma> o \<tau>)" 
+unfolding small_def using supp_o by (metis countable_Un_iff countable_subset)
+
+lemma supp_inv[simp]: "bij \<sigma> \<Longrightarrow> small \<sigma> \<Longrightarrow> supp (inv \<sigma>) = supp \<sigma>" 
+unfolding supp_def by (metis bij_inv_eq_iff)
+lemma small_inv[simp]: "bij \<sigma> \<Longrightarrow> small (inv \<sigma>) \<longleftrightarrow> small \<sigma>" 
+unfolding small_def by (metis bij_betw_inv_into inv_inv_eq small_def supp_inv)
+
+(* declare bij_id[intro] *)
+lemmas bij_id'[simp,intro]=bij_id[unfolded id_def]
+(* declare bij_comp[simp] *)
+(* declare bij_imp_bij_inv[simp] *)
+
+lemmas bij_inv_id1 = inv_o_simp2 (* [simp] *) (* : "bij f \<Longrightarrow> f o inv f = id" unfolding fun_eq_iff *)
+ (*  by (simp add: bij_def surj_iff) *)
+lemmas bij_inv_id2 = inv_o_simp1 
+(*[simp]: "bij f \<Longrightarrow> inv f o f = id" unfolding fun_eq_iff 
+by (simp add: bij_def surj_iff) *)
+
+(**************************)
+(* 2. The starting MN-monad / pre-(co)datatype *)
 
 typedecl Gbd_type
 consts Gbd :: "Gbd_type rel"
@@ -61,13 +122,13 @@ lemma IImsupp_bound[simp]:
   unfolding IImsupp_def IImsupp'_def
   by (auto simp: Un_bound UN_bound)
 
-typedecl ('a1, 'a2, 'x1, 'x2) G
-consts Gsub :: "('a1 :: var \<Rightarrow> 'a1) \<Rightarrow> ('a2 :: var \<Rightarrow> 'a2) \<Rightarrow> ('a1, 'a2, 'x1, 'x2) G \<Rightarrow> ('a1, 'a2, 'x1, 'x2) G"
-consts GVrs1 :: "('a1 :: var, 'a2 :: var, 'x1, 'x2) G \<Rightarrow> 'a1 set"
-consts GVrs2 :: "('a1 :: var, 'a2 :: var, 'x1, 'x2) G \<Rightarrow> 'a2 set"
-consts Gmap :: "('x1 \<Rightarrow> 'x1') \<Rightarrow> ('x2 \<Rightarrow> 'x2') \<Rightarrow> ('a1, 'a2, 'x1, 'x2) G \<Rightarrow> ('a1, 'a2, 'x1', 'x2') G"
-consts GSupp1 :: "('a1 :: var, 'a2 :: var, 'x1, 'x2) G \<Rightarrow> 'x1 set"
-consts GSupp2 :: "('a1 :: var, 'a2 :: var, 'x1, 'x2) G \<Rightarrow> 'x2 set"
+typedecl ('a1, 'a2, 'c1, 'c2) G
+consts Gsub :: "('a1 :: var \<Rightarrow> 'a1) \<Rightarrow> ('a2 :: var \<Rightarrow> 'a2) \<Rightarrow> ('a1, 'a2, 'c1, 'c2) G \<Rightarrow> ('a1, 'a2, 'c1, 'c2) G"
+consts GVrs1 :: "('a1 :: var, 'a2 :: var, 'c1, 'c2) G \<Rightarrow> 'a1 set"
+consts GVrs2 :: "('a1 :: var, 'a2 :: var, 'c1, 'c2) G \<Rightarrow> 'a2 set"
+consts Gmap :: "('c1 \<Rightarrow> 'c1') \<Rightarrow> ('c2 \<Rightarrow> 'c2') \<Rightarrow> ('a1, 'a2, 'c1, 'c2) G \<Rightarrow> ('a1, 'a2, 'c1', 'c2') G"
+consts GSupp1 :: "('a1 :: var, 'a2 :: var, 'c1, 'c2) G \<Rightarrow> 'c1 set"
+consts GSupp2 :: "('a1 :: var, 'a2 :: var, 'c1, 'c2) G \<Rightarrow> 'c2 set"
 
 setup \<open>Sign.mandatory_path "G"\<close>
 
@@ -135,6 +196,10 @@ definition Gren ::
 lemma GVrs2_bound[simp]: "|GVrs2 (u::('a :: var, 'a, 'e, 'e) G)| <o |UNIV :: 'a set|"
   by (rule ordLess_ordLeq_trans[OF G.Vrs_bd(2) large'])
 
+
+(**************************)
+(* 3. Generalized Nominal Assumptions *)
+
 locale Nominal = 
   fixes Eperm :: "('a :: var \<Rightarrow> 'a) \<Rightarrow> 'e \<Rightarrow> 'e"
   and EVrs :: "'e \<Rightarrow> 'a set"
@@ -164,6 +229,7 @@ lemma EVrs_bound[simp]: "|EVrs (x :: 'e)| <o |UNIV :: 'a set|"
 
 end
 
+(* relativized nominal :*)
 locale NominalRel = 
   fixes Pvalid :: "'e \<Rightarrow> bool"
   and Pperm :: "('a :: var \<Rightarrow> 'a) \<Rightarrow> 'e \<Rightarrow> 'e"
@@ -177,7 +243,11 @@ locale NominalRel =
    Pperm \<sigma> (Pperm \<tau> e) = Pperm (\<sigma> o \<tau>) e"
   and Eperm_cong_id:
   "\<And>\<sigma> e. bij (\<sigma> :: 'a :: var \<Rightarrow> 'a) \<Longrightarrow> |supp \<sigma>| <o |UNIV :: 'a set| \<Longrightarrow> Pvalid e \<Longrightarrow>
-   (\<And>a. a \<in> PVrs e \<Longrightarrow> \<sigma> a = a) \<Longrightarrow> Pperm \<sigma> e = e"
+   (\<And>a. a \<in> PVrs e \<Longrightarrow> \<sigma> a = a) \<Longrightarrow> Pperm \<sigma> e = e" 
+
+
+(**************************)
+(* 4. Expression-Like Entities *)
 
 locale Expression = Nominal +
   fixes Ector :: "('a :: var, 'a, 'e, 'e) G \<Rightarrow> 'e"
